src/KernelMode.v
@@ -11,17 +11,17 @@ Section KernelMode.
   (** # Kernel Mode
 
 At each moment of execution VM is either in **kernel** or in **user mode**. Some
-instructions are only allowed in kernel mode; executing them in user mode results in executing [%%OpPanic] instead.
+instructions are only allowed in kernel mode; executing them in user mode results in executing [%OpPanic] instead.
 
 Current mode is determined by the address of the currently executed contract: if
-the address is in range from 0 to [%%KERNEL_MODE_MAXADDR_LIMIT] (exclusive),
+the address is in range from 0 to [%KERNEL_MODE_MAXADDR_LIMIT] (exclusive),
 current mode is kernel, otherwise current mode is user mode. *)
   Definition KERNEL_MODE_MAXADDR_LIMIT : contract_address := 2^16.
 
   Definition addr_is_kernel (addr:contract_address) : bool :=
     addr < KERNEL_MODE_MAXADDR_LIMIT.
 
-(** Current contract's address can be obtained from the active external frame in [%%callstack].
+(** Current contract's address can be obtained from the active external frame in [%callstack].
 Topmost external frame (active frame) is obtained through [%active_extframe], it contains the current contract's address in its field [%ecf_this_address]. *)
 
   (** The list of instructions requiring kernel mode is encoded by the
